pcuic/theories/PCUICTyping.v
@@ -401,7 +401,8 @@ Definition branches_size {cf} {Σ Γ ci mdecl idecl p ps ptm brs}
       (Nat.max (typing_size _ _ _ _ p.2.2.1) (typing_size _ _ _ _ p.2.2.2))) a).
 
 Section CtxInstSize.
-  Context {cf} (typing_size : forall {Σ Γ t T}, Σ ;;; Γ |- t : T -> size).
+  Context {cf} (typing : global_env_ext -> context -> term -> term -> Type)
+  (typing_size : forall {Σ Γ t T}, typing Σ Γ t T -> size).
 
   Fixpoint ctx_inst_size {Σ Γ args Δ} (c : ctx_inst typing Σ Γ args Δ) : size :=
   match c with
@@ -943,7 +944,7 @@ Proof.
         ++ eapply (Hwf _ a0). rewrite /predctx; simpl. lia.
         ++ clear -c1 X14.
           assert (forall (Γ' : context) (t T : term) (Hty : Σ;;; Γ' |- t : T),
-            typing_size Hty <= ctx_inst_size (@typing_size _) c1 ->
+            typing_size Hty <= ctx_inst_size _ (@typing_size _) c1 ->
             P Σ Γ' t T).
           { intros. eapply (X14 _ _ _ Hty). simpl. lia. }
           clear -X c1.
